STLC_SuccNat/LR.v
@@ -4,7 +4,7 @@ Require Import Lifted_STLC_SuccNat.
 Import ListNotations.
 Require Import Norm Lifted_Norm Derivation.
 
-Fixpoint LR (cfg:feat_config) (T:ty) (t:tm) (t':tm') : Prop :=
+Fixpoint LR `{NatOp} (cfg:feat_config) (T:ty) (t:tm) (t':tm') : Prop :=
   has_type empty t T /\ has_type' empty t' (lift_ty T) /\
   match T with
   | Nat => exists r r',
@@ -20,14 +20,14 @@ Fixpoint LR (cfg:feat_config) (T:ty) (t:tm) (t':tm') : Prop :=
 	          derive' cfg r' = Some r
   end.
 
-Lemma LR_typable_empty : forall {cfg} {T} {t} {t'},
+Lemma LR_typable_empty `{NatOp}: forall {cfg} {T} {t} {t'},
   LR cfg T t t' ->
   has_type empty t T /\ has_type' empty t' (lift_ty T).
 Proof.
   intros.
-  destruct T; unfold LR in H; split;
-    try (destruct H as [H _]; assumption);
-    destruct H as [_ [H _] ]; assumption.
+  destruct T; unfold LR in H0; split;
+    try (destruct H0 as [H0 _]; assumption);
+    destruct H0 as [_ [H0 _] ]; assumption.
 Qed.
 
 (* This proof depends on normalization
@@ -42,17 +42,18 @@ Qed.
    This implies that ever well typed term halts
    (normalization)
 *)
-Lemma LR_halts: forall {cfg} {T} {t} {t'},
+Lemma LR_halts `{NatOp}: forall {cfg} {T} {t} {t'},
   LR cfg T t t' -> halts t /\ halts' t'.
 Proof.
   intros. split; [eapply normalization| eapply normalization'];
   eapply LR_typable_empty; eassumption.
 Qed.
 
-Lemma step_preserves_LR : forall T cfg t1 t2 t', (step t1 t2) -> LR cfg T t1 t' -> LR cfg T t2 t'.
+Lemma step_preserves_LR `{NatOp}: forall T cfg t1 t2 t',
+  (step t1 t2) -> LR cfg T t1 t' -> LR cfg T t2 t'.
 Proof.
  induction T;  intros cfg t1 t2 t' E Rt; unfold R; fold R; unfold R in Rt; fold R in Rt;
-               destruct Rt as [Hty [Hty' H] ].
+               destruct Rt as [Hty [Hty' H0]].
   (* Arrow *)
   - split; [|split].
     eapply preservation; eauto.
@@ -61,39 +62,40 @@ Proof.
     intros.
     eapply IHT2.
     apply ST_App1. apply E.
-    apply H. assumption.
+    apply H0. assumption.
   (* Nat *)
   - split; [|split]; auto.
     eapply preservation; eauto.
-    destruct H as [r [r' [Hsnf [Hsnf' Hd] ] ] ].
+    destruct H0 as [r [r' [Hsnf [Hsnf' Hd] ] ] ].
     exists r, r'. split; [|split]; auto.
     clear Hsnf' Hd Hty Hty'.
     destruct Hsnf as [Hms Hv].
     split; auto.
     inversion Hms; subst.
     exfalso; apply Hv; eauto.
-    apply (determinism _ _ _ H) in E.
+    apply (determinism _ _ _ H0) in E.
     rewrite E in *.
     assumption.
   (* NatList *)
   - split; [|split]; auto.
     eapply preservation; eauto.
-    destruct H as [r [r' [Hsnf [Hsnf' Hd]]]].
+    destruct H0 as [r [r' [Hsnf [Hsnf' Hd]]]].
     exists r, r'. split; [|split]; auto.
     clear Hsnf' Hd Hty Hty'.
     destruct Hsnf as [Hms Hv].
     split; auto.
     inversion Hms; subst.
     exfalso; apply Hv; eauto.
-    apply (determinism _ _ _ H) in E.
+    apply (determinism _ _ _ H0) in E.
     rewrite E in *.
     assumption.
 Qed.
 
-Lemma step'_preserves_LR : forall T cfg t t1' t2', (step' t1' t2') -> LR cfg T t t1' -> LR cfg T t t2'.
+Lemma step'_preserves_LR `{NatOp}: forall T cfg t t1' t2',
+  (step' t1' t2') -> LR cfg T t t1' -> LR cfg T t t2'.
 Proof.
  induction T;  intros cfg t t1' t2' E Rt; unfold R; fold R; unfold R in Rt; fold R in Rt;
-               destruct Rt as [Hty [Hty' H] ].
+               destruct Rt as [Hty [Hty' H0]].
   (* Arrow *)
   - split; [|split].
     assumption.
@@ -102,42 +104,42 @@ Proof.
     intros.
     eapply IHT2.
     apply ST_App1'. apply E.
-    apply H. assumption.
+    apply H0. assumption.
   (* Nat *)
   - split; [|split]; auto.
     eapply preservation'; eauto.
-    destruct H as [r [r' [Hsnf [Hsnf' Hd] ] ] ].
+    destruct H0 as [r [r' [Hsnf [Hsnf' Hd]]]].
     exists r, r'. split; [|split]; auto.
     clear Hsnf Hd Hty Hty'.
     destruct Hsnf' as [Hms' Hv'].
     split; auto.
     inversion Hms'; subst.
     exfalso; apply Hv'; eauto.
-    apply (determinism' _ _ _ H) in E.
+    apply (determinism' _ _ _ H0) in E.
     rewrite E in *.
     assumption.
   (* NatList *)
   - split; [|split]; auto.
     eapply preservation'; eauto.
-    destruct H as [r [r' [Hsnf [Hsnf' Hd]]]].
+    destruct H0 as [r [r' [Hsnf [Hsnf' Hd]]]].
     exists r, r'. split; [|split]; auto.
     clear Hsnf Hd Hty Hty'.
     destruct Hsnf' as [Hms' Hv'].
     split; auto.
     inversion Hms'; subst.
     exfalso; apply Hv'; eauto.
-    apply (determinism' _ _ _ H) in E.
+    apply (determinism' _ _ _ H0) in E.
     rewrite E in *.
     assumption.
 Qed.
 
-Lemma step_preserves_LR' : forall T cfg t1 t2 t',
+Lemma step_preserves_LR' `{NatOp}: forall T cfg t1 t2 t',
   has_type empty t1 T -> 
   (step t1 t2) ->
   LR cfg T t2 t' -> LR cfg T t1 t'.
 Proof.
  induction T;  intros cfg t1 t2 t' HT E Rt; unfold R; fold R; unfold R in Rt; fold R in Rt;
-               destruct Rt as [Hty [Hty' H] ].
+               destruct Rt as [Hty [Hty' H0]].
   (* Arrow *)
   - split; [|split].
     auto.
@@ -148,10 +150,10 @@ Proof.
     eapply T_App. eauto.
     eapply LR_typable_empty; eauto.
     apply ST_App1. apply E.
-    apply H. assumption.
+    apply H0. assumption.
   (* Nat *)
   - split; [|split]; auto.
-    destruct H as [r [r' [Hsnf [Hsnf' Hd] ] ] ].
+    destruct H0 as [r [r' [Hsnf [Hsnf' Hd]]]].
     exists r, r'. split; [|split]; auto.
     clear Hsnf' Hd Hty Hty'.
     destruct Hsnf as [Hms Hv].
@@ -159,7 +161,7 @@ Proof.
     inversion Hms; subst; eauto.
   (* NatList *)
   - split; [|split]; auto.
-    destruct H as [r [r' [Hsnf [Hsnf' Hd] ] ] ].
+    destruct H0 as [r [r' [Hsnf [Hsnf' Hd]]]].
     exists r, r'. split; [|split]; auto.
     clear Hsnf' Hd Hty Hty'.
     destruct Hsnf as [Hms Hv].
@@ -167,13 +169,13 @@ Proof.
     inversion Hms; subst; eauto.
 Qed.
 
-Lemma step'_preserves_LR' : forall T cfg t t1' t2',
+Lemma step'_preserves_LR' `{NatOp}: forall T cfg t t1' t2',
   has_type' empty t1' (lift_ty T) -> 
   (step' t1' t2') ->
   LR cfg T t t2' -> LR cfg T t t1'.
 Proof.
  induction T;  intros cfg t t1' t2' HT E Rt; unfold R; fold R; unfold R in Rt; fold R in Rt;
-               destruct Rt as [Hty [Hty' H] ].
+               destruct Rt as [Hty [Hty' H0]].
   (* Arrow *)
   - split; [|split].
     auto.
@@ -184,10 +186,10 @@ Proof.
     eapply T_App'. eauto.
     eapply LR_typable_empty; eauto.
     apply ST_App1'. apply E.
-    apply H. assumption.
+    apply H0. assumption.
   (* Nat *)
   - split; [|split]; auto.
-    destruct H as [r [r' [Hsnf [Hsnf' Hd] ] ] ].
+    destruct H0 as [r [r' [Hsnf [Hsnf' Hd]]]].
     exists r, r'. split; [|split]; auto.
     clear Hsnf Hd Hty Hty'.
     destruct Hsnf' as [Hms' Hv'].
@@ -195,7 +197,7 @@ Proof.
     inversion Hms'; subst; eauto.
   (* NatList *)
   - split; [|split]; auto.
-    destruct H as [r [r' [Hsnf [Hsnf' Hd] ] ] ].
+    destruct H0 as [r [r' [Hsnf [Hsnf' Hd]]]].
     exists r, r'. split; [|split]; auto.
     clear Hsnf Hd Hty Hty'.
     destruct Hsnf' as [Hms' Hv'].
@@ -203,61 +205,61 @@ Proof.
     inversion Hms'; subst; eauto.
 Qed.
 
-Lemma mstep_preserves_LR': forall T cfg t1 t2 t',
+Lemma mstep_preserves_LR' `{NatOp}: forall T cfg t1 t2 t',
   has_type empty t1 T ->
   multi step t1 t2 ->
   LR cfg T t2 t' -> LR cfg T t1 t'.
 Proof.
-  intros. induction H0.
+  intros. induction H1.
   - assumption.
-  - apply (preservation _ _ _ H) in H0 as H3.
-    apply (IHmulti H3) in H1.
+  - apply (preservation _ _ _ H0) in H1 as H4.
+    apply (IHmulti H4) in H2.
     eapply step_preserves_LR'; eauto.
 Qed.
 
-Lemma mstep_preserves_LR: forall T cfg t1 t2 t',
+Lemma mstep_preserves_LR `{NatOp}: forall T cfg t1 t2 t',
   multi step t1 t2 ->
   LR cfg T t1 t' -> LR cfg T t2 t'.
 Proof.
-  intros. induction H.
+  intros. induction H0.
   - assumption.
   - apply IHmulti.
     eapply step_preserves_LR; eauto.
 Qed.
 
-Lemma mstep'_preserves_LR': forall T cfg t t1' t2',
+Lemma mstep'_preserves_LR' `{NatOp}: forall T cfg t t1' t2',
   has_type' empty t1' (lift_ty T) ->
   multi step' t1' t2' ->
   LR cfg T t t2' -> LR cfg T t t1'.
 Proof.
-  intros. induction H0.
+  intros. induction H1.
   - assumption.
-  - apply (preservation' _ _ _ H) in H0 as H3.
-    apply (IHmulti H3) in H1.
+  - apply (preservation' _ _ _ H0) in H1 as H4.
+    apply (IHmulti H4) in H2.
     eapply step'_preserves_LR'; eauto.
 Qed.
 
-Lemma mstep'_preserves_LR: forall T cfg t t1' t2',
+Lemma mstep'_preserves_LR `{NatOp}: forall T cfg t t1' t2',
   multi step' t1' t2' ->
   LR cfg T t t1' -> LR cfg T t t2'.
 Proof.
-  intros. induction H.
+  intros. induction H0.
   - assumption.
   - apply IHmulti.
     eapply step'_preserves_LR; eauto.
 Qed.
 
-Lemma mstep_mstep'__preserves_LR: forall T cfg t1 t2 t1' t2',
+Lemma mstep_mstep'__preserves_LR `{NatOp}: forall T cfg t1 t2 t1' t2',
   multi step t1 t2 ->
   multi step' t1' t2' ->
   LR cfg T t1 t1' -> LR cfg T t2 t2'.
 Proof.
   intros.
-  apply (mstep'_preserves_LR _ _ _ _ t2') in H1; auto.
-  apply (mstep_preserves_LR _ _ _ t2) in H1; auto.
+  apply (mstep'_preserves_LR _ _ _ _ t2') in H2; auto.
+  apply (mstep_preserves_LR _ _ _ t2) in H2; auto.
 Qed.
 
-Lemma mstep_mstep'__preserves_LR': forall T cfg t1 t2 t1' t2',
+Lemma mstep_mstep'__preserves_LR' `{NatOp}: forall T cfg t1 t2 t1' t2',
   has_type empty t1 T ->
   has_type' empty t1' (lift_ty T) ->
   multi step t1 t2 ->
@@ -265,13 +267,13 @@ Lemma mstep_mstep'__preserves_LR': forall T cfg t1 t2 t1' t2',
   LR cfg T t2 t2' -> LR cfg T t1 t1'.
 Proof.
   intros.
-  apply (preservation'_multi _ _ _ H0) in H2 as H4.
-  apply (mstep'_preserves_LR' _ _ _ t1') in H3; auto.
-  apply (preservation_multi _ _ _ H) in H1 as H5.
-  apply (mstep_preserves_LR' _ _ t1) in H3; auto.
+  apply (preservation'_multi _ _ _ H1) in H3 as H5.
+  apply (mstep'_preserves_LR' _ _ _ t1') in H4; auto.
+  apply (preservation_multi _ _ _ H0) in H2 as H6.
+  apply (mstep_preserves_LR' _ _ t1) in H4; auto.
 Qed.
 
-Definition commutes T cfg analysis := forall spl p r r',
+Definition commutes `{NatOp} T cfg analysis := forall spl p r r',
   has_type' empty spl (lift_ty T) ->
   derive' cfg spl = Some p ->
   step_normal_form_of (app analysis p) r ->
@@ -284,7 +286,7 @@ Definition base_ty T := T = Nat \/ T = NatList.
     expressiviness of the Lifted Language. A Variational Natural
     is represented by a List with only one value. *)
 
-Lemma soundness: forall T cfg analysis,
+Lemma soundness `{NatOp}: forall T cfg analysis,
   LR cfg (Arrow NatList T) analysis (lift analysis) ->
     commutes NatList cfg analysis.
 Proof.
@@ -316,7 +318,7 @@ Proof.
 Abort.
 
 
-Lemma soundness: forall T cfg analysis,
+Lemma soundness `{NatOp}: forall T cfg analysis,
   base_ty T ->
   LR cfg (Arrow T T) analysis (lift analysis) ->
     commutes T cfg analysis.
@@ -325,7 +327,7 @@ Proof.
   unfold LR in HLR. destruct HLR as [_ [_ HLR]].
   specialize HLR with (arg:=p) (arg':=spl).
   destruct Hbt; subst; destruct HLR;
-    try (destruct H0 as [_ [r0 [r0' [Hsnf0 [Hsnf0' Hd0']]]]];
+    try (destruct H1 as [_ [r0 [r0' [Hsnf0 [Hsnf0' Hd0']]]]];
          apply (normal_forms_unique _ _ _ Hsnf0) in Hsnf;
          apply (normal_forms'_unique _ _ _ Hsnf0') in Hsnf';
          subst; assumption).
@@ -357,7 +359,7 @@ Qed.
 
 Require Import Environments.
 
-Inductive instantiation : feat_config -> tass -> env -> env' -> Prop :=
+Inductive instantiation `{NatOp}: feat_config -> tass -> env -> env' -> Prop :=
   | V_nil : forall cfg, instantiation cfg [] [] []
   | V_cons : forall cfg x T v v' c e e',
     instantiation cfg c e e'->
@@ -365,7 +367,7 @@ Inductive instantiation : feat_config -> tass -> env -> env' -> Prop :=
     LR cfg T v v' ->
     instantiation cfg ((x,T)::c) ((x,v)::e) ((x,v')::e').
 
-Lemma instantiation_domains_match: forall {cfg} {c} {e} {e'},
+Lemma instantiation_domains_match `{NatOp}: forall {cfg} {c} {e} {e'},
   instantiation cfg c e e'->
   forall {x} {T},
     lookup x c = Some T -> 
@@ -378,7 +380,7 @@ Proof.
     destruct (eqb x x0); eauto.
 Qed.
 
-Lemma instantiation_LR : forall cfg c e e',
+Lemma instantiation_LR `{NatOp}: forall cfg c e e',
   instantiation cfg c e e' ->
   forall x t t' T,
     lookup x c = Some T ->
@@ -398,7 +400,7 @@ Proof.
     + eauto.
 Qed.
 
-Lemma instantiation_env_closed: forall cfg c e e',
+Lemma instantiation_env_closed `{NatOp}: forall cfg c e e',
   instantiation cfg c e e' -> closed_env e /\ closed'_env' e'.
 Proof.
   intros cfg c e e' Hinst.
@@ -418,17 +420,17 @@ Proof.
       eassumption.
 Qed.
 
-Lemma msubst_preserves_typing : forall cfg c e e',
+Lemma msubst_preserves_typing `{NatOp}: forall cfg c e e',
   instantiation cfg c e e' ->
   forall Gamma t S, has_type (mupdate Gamma c) t S ->
   has_type Gamma (msubst e t) S.
 Proof.
-    intros cfg c e e' H. induction H; intros.
-    simpl in H. simpl. auto.
-    simpl in H3.  simpl.
+    intros cfg c e e' H0. induction H0; intros.
+    simpl in H0. simpl. auto.
+    simpl in H4.  simpl.
     apply IHinstantiation.
     eapply substitution_preserves_typing; eauto.
-    apply (LR_typable_empty H2).
+    apply (LR_typable_empty H3).
 Qed.
 
 Fixpoint lift_tass (c:tass) : tass' :=
@@ -446,21 +448,21 @@ Proof.
   simpl. f_equal. assumption.
 Qed.
 
-Lemma msubst'_preserves_typing : forall cfg c e e',
+Lemma msubst'_preserves_typing `{NatOp}: forall cfg c e e',
   instantiation cfg c e e' ->
   forall Gamma' t' S', has_type' (mupdate' Gamma' (lift_tass c)) t' S' ->
   has_type' Gamma' (msubst' e' t') S'.
 Proof.
-    intros cfg c e e' H. induction H; intros.
-    simpl in H. simpl. auto.
-    simpl in H2. simpl.
+    intros cfg c e e' H0. induction H0; intros.
+    simpl in H0. simpl. auto.
+    simpl in H3. simpl.
     apply IHinstantiation.
-    simpl in H3.
+    simpl in H4.
     eapply substitution_preserves_typing'; eauto.
-    apply (LR_typable_empty H2).
+    apply (LR_typable_empty H3).
 Qed.
 
-Lemma instantiation_drop : forall cfg c env env',
+Lemma instantiation_drop `{NatOp}: forall cfg c env env',
     instantiation cfg c env env' ->
     forall x, instantiation cfg (drop x c) (drop x env) (drop x env').
 Proof.
@@ -504,7 +506,7 @@ Qed.
 
 (* Pattern matching acts like lambda abstraction because
    evaluating it envolves beta reduction. *)
-Lemma completeness: forall c env env' t T cfg,
+Lemma completeness `{NatOp}: forall c env env' t T cfg,
   has_type (mupdate empty c)  t T ->
   instantiation cfg c env env' ->
   LR cfg T (msubst env t) (msubst' env' (lift t)).
@@ -519,8 +521,8 @@ Proof.
   generalize dependent c.
   induction HT; simpl; intros.
   - (* T_Var *)
-    rewrite H0 in H.
-    destruct (instantiation_domains_match V H) as [t [P [t' P'] ] ].
+    rewrite H1 in H0.
+    destruct (instantiation_domains_match V H0) as [t [P [t' P'] ] ].
     eapply instantiation_LR; eauto.
     * rewrite msubst_var.
       rewrite P; reflexivity.
@@ -537,7 +539,7 @@ Proof.
       intros.
       unfold update, t_update. rewrite mupdate_drop. destruct (eqb_spec x x0).
       + auto.
-      + rewrite H.
+      + rewrite H0.
         clear - c n. induction c.
         simpl. apply eqb_neq in n; rewrite n; auto.
         simpl. destruct a.  unfold update, t_update.
@@ -554,7 +556,7 @@ Proof.
       rewrite lift_tass_drop, mupdate'_drop.
       destruct (eqb_spec x x0).
       + auto.
-      + rewrite H.
+      + rewrite H0.
         clear - c n. induction c.
         simpl. apply eqb_neq in n; rewrite n; auto.
         simpl. destruct a. simpl.
@@ -562,8 +564,8 @@ Proof.
         destruct (String.eqb s x0); auto. }
       split; [|split]; auto.
       intros.
-      destruct (LR_halts H0) as [ [v [P Q] ] [v' [P' Q'] ] ].
-      pose proof (mstep_mstep'__preserves_LR _ _ _ _ _ _ P P' H0).
+      destruct (LR_halts H1) as [ [v [P Q] ] [v' [P' Q'] ] ].
+      pose proof (mstep_mstep'__preserves_LR _ _ _ _ _ _ P P' H1).
       apply mstep_mstep'__preserves_LR' with (msubst ((x,v)::env0) t) (msubst' ((x,v')::env0') (lift t)).
       { eapply T_App; eauto.
         eapply LR_typable_empty; eauto. }
@@ -575,7 +577,7 @@ Proof.
             simpl.  rewrite subst_msubst.
             eapply ST_AppAbs; eauto.
             eapply typable_empty__closed.
-            apply (LR_typable_empty H1).
+            apply (LR_typable_empty H2).
             eapply instantiation_env_closed; eauto. }
       { eapply multi_step'_trans. eapply multistep'_app2'; eauto.
             eapply multi_step with (y:= (msubst' ((x, v') :: env0') (lift t)));
@@ -583,17 +585,17 @@ Proof.
             simpl.  rewrite subst'_msubst'.
             eapply ST_AppAbs'; eauto.
             eapply typable_empty__closed'.
-            apply (LR_typable_empty H1).
+            apply (LR_typable_empty H2).
             eapply instantiation_env_closed; eauto.  }
       eapply (IHHT ((x,T2)::c)).
         intros. unfold update, t_update, lookup. destruct (String.eqb x x0); auto.
       constructor; auto.
   - (* T_App *)
     rewrite msubst_app, msubst'_app'.
-    pose proof (IHHT1 c H env0 env0' V).
-    unfold LR in H0; fold LR in H0.
-    destruct H0 as [_ [_ HLR] ].
-    pose proof (IHHT2 c H env0 env0' V).
+    pose proof (IHHT1 c H0 env0 env0' V).
+    unfold LR in H1; fold LR in H1.
+    destruct H1 as [_ [_ HLR]].
+    pose proof (IHHT2 c H0 env0 env0' V).
     auto.
   - (* T_Const *)
     split; [|split].
@@ -609,7 +611,7 @@ Proof.
         | intros [x contra]; inversion contra].
     + reflexivity.
   - (* T_Succ *)
-    destruct (IHHT c H env0 env0' V) as [HT0 [HT' [r [r' [ [Hms Hnf] [ [Hms' _] Hd]]]]]].
+    destruct (IHHT c H0 env0 env0' V) as [HT0 [HT' [r [r' [ [Hms Hnf] [ [Hms' _] Hd]]]]]].
     split; [|split].
     rewrite msubst_succ. auto.
     rewrite msubst'_succ'. auto.
@@ -639,36 +641,36 @@ Proof.
       try solve_by_inverts 1.
       injection Hd as Hd; auto.
   - (* T_Add *)
-    rewrite msubst_add, msubst'_add'.
-    destruct (IHHT1 c H env0 env0' V) as [HT11 [HT1' [r1 [r1' [[Hms1 _] [[Hms1' _] Hd1]]]]]].
-    destruct (IHHT2 c H env0 env0' V) as [HT22 [HT2' [r2 [r2' [[Hms2 _] [[Hms2' _] Hd2]]]]]].
+    rewrite msubst_op, msubst'_op'.
+    destruct (IHHT1 c H0 env0 env0' V) as [HT11 [HT1' [r1 [r1' [[Hms1 _] [[Hms1' _] Hd1]]]]]].
+    destruct (IHHT2 c H0 env0 env0' V) as [HT22 [HT2' [r2 [r2' [[Hms2 _] [[Hms2' _] Hd2]]]]]].
     split; [|split]; auto.
     pose proof (preservation_multi _ _ _ HT11 Hms1).
     pose proof (preservation'_multi _ _ _ HT1' Hms1').
     pose proof (derive'_value _ _ _ Hd1) as [].
-    apply (canonical_forms_nat _ H0) in H2 as [n1]; subst.
-    apply (canonical_forms_nat' _ H1) in H3 as [n1']; subst.
-    clear H0 H1.
+    apply (canonical_forms_nat _ H1) in H3 as [n1]; subst.
+    apply (canonical_forms_nat' _ H2) in H4 as [n1']; subst.
+    clear H1 H2.
     pose proof (preservation_multi _ _ _ HT22 Hms2).
     pose proof (derive'_value _ _ _ Hd2) as [].
     pose proof (preservation'_multi _ _ _ HT2' Hms2').
-    apply (canonical_forms_nat _ H0) in H1 as [n2]; subst.
-    apply (canonical_forms_nat' _ H3) in H2 as [n2']; subst.
-    clear H0 H3.
-    exists (const (n1 + n2)), (const' (app_binop Nat.add n1' n2'));
+    apply (canonical_forms_nat _ H1) in H2 as [n2]; subst.
+    apply (canonical_forms_nat' _ H4) in H3 as [n2']; subst.
+    clear H1 H4.
+    exists (const (nat_op n1 n2)), (const' (app_binop nat_op n1' n2'));
     repeat split.
     + eapply multi_step_trans.
-      apply multistep_add1; eassumption.
+      apply multistep_op1; eassumption.
       eapply multi_step_trans.
-      apply multistep_add2; eauto.
-      eapply multi_step. apply ST_AddConst.
+      apply multistep_op2; eauto.
+      eapply multi_step. apply ST_OpConst.
       apply multi_refl.
     + intros [x contra]; inversion contra.
     + eapply multi_step'_trans.
-      apply multistep'_add1'; eassumption.
+      apply multistep'_op1'; eassumption.
       eapply multi_step'_trans.
-      apply multistep'_add2'; eauto.
-      eapply multi_step. apply ST_AddConst'.
+      apply multistep'_op2'; eauto.
+      eapply multi_step. apply ST_OpConst'.
       apply multi_refl.
     + intros [x contra]; inversion contra.
     + simpl.
@@ -695,17 +697,17 @@ Proof.
     + reflexivity.
   - (* T_Cons *)
     rewrite msubst_cons, msubst'_cons'.
-    pose proof (IHHT1 c H env0 env0' V).
-    unfold LR in H0; fold LR in H0.
-    destruct H0 as [Hty1 [Hty1' HLR]].
-    pose proof (IHHT2 c H env0 env0' V).
+    pose proof (IHHT1 c H0 env0 env0' V).
+    unfold LR in H1; fold LR in H1.
+    destruct H1 as [Hty1 [Hty1' HLR]].
+    pose proof (IHHT2 c H0 env0 env0' V).
     clear IHHT1 IHHT2.
     split; [|split];
     try (constructor; auto;
-    destruct (LR_typable_empty H0) as [H1 H2]; auto).
+    destruct (LR_typable_empty H1) as [H2 H3]; auto).
     destruct HLR as [r1 [r1' [[Hms1 Hnf1] [[Hms1' Hnf1'] Hd1]]]].
-    unfold LR in H0.
-    destruct H0 as [_ [_ [r2 [r2' [[Hms2 Hnf2] [[Hms2' Hnf2'] Hd2]]]]]].
+    unfold LR in H1.
+    destruct H1 as [_ [_ [r2 [r2' [[Hms2 Hnf2] [[Hms2' Hnf2'] Hd2]]]]]].
     eexists; eexists.
     split; [|split].
     + split. eapply multi_step_trans.
@@ -739,7 +741,6 @@ Proof.
       reflexivity.
   - (* T_Case *)
     rewrite msubst_case, msubst'_case'.
-
     assert (Hty: has_type empty (case (msubst env0 t1) (msubst env0 tnil) x y
      (msubst (drop y (drop x env0)) tcons)) (T)).
     { apply T_Case.
@@ -756,7 +757,7 @@ Proof.
       unfold update, t_update. repeat (rewrite mupdate_drop).
       destruct (eqb_spec x x0); destruct (eqb_spec y x0);
         try auto.
-        rewrite H.
+        rewrite H0.
         clear - c n n0. induction c.
         simpl. apply eqb_neq in n, n0; try rewrite n, n0; auto.
         simpl. destruct a.  unfold update, t_update.
@@ -768,50 +769,48 @@ Proof.
        eapply context'_invariance. apply (lifting_types _ _ _ HT1).
        intros. rewrite <- mupdate'_lookup.
        unfold lift_context. unfold lift_tass.
-       rewrite H. clear - c. induction c. auto.
+       rewrite H0. clear - c. induction c. auto.
          destruct a. simpl.
          destruct (String.eqb s x0); auto.
-
-      eapply msubst'_preserves_typing. eassumption.
-      eapply context'_invariance. apply (lifting_types _ _ _ HT2).
-      intros. rewrite <- mupdate'_lookup.
-      unfold lift_context. unfold lift_tass.
-       rewrite H. clear - c. induction c. auto.
-         destruct a. simpl.
-      destruct (String.eqb s x0); auto.
-
-      eapply msubst'_preserves_typing.
-      repeat (apply instantiation_drop); eauto.
-      eapply context'_invariance. apply (lifting_types _ _ _ HT3).
-      intros.
-      unfold update, t_update, lift_context.
-      repeat (rewrite lift_tass_drop, mupdate'_drop).
-      destruct (eqb_spec x x0); destruct (eqb_spec y x0);
+       eapply msubst'_preserves_typing. eassumption.
+       eapply context'_invariance. apply (lifting_types _ _ _ HT2).
+       intros. rewrite <- mupdate'_lookup.
+       unfold lift_context. unfold lift_tass.
+       rewrite H0. clear - c. induction c. auto.
+       destruct a. simpl.
+       destruct (String.eqb s x0); auto.
+       eapply msubst'_preserves_typing.
+       repeat (apply instantiation_drop); eauto.
+       eapply context'_invariance. apply (lifting_types _ _ _ HT3).
+       intros.
+       unfold update, t_update, lift_context.
+       repeat (rewrite lift_tass_drop, mupdate'_drop).
+       destruct (eqb_spec x x0); destruct (eqb_spec y x0);
         try auto.
-        rewrite H.
+        rewrite H0.
         clear - c n n0. induction c.
         simpl. apply eqb_neq in n, n0; try rewrite n, n0; auto.
         destruct a. simpl. unfold update, t_update.
         destruct (String.eqb s x0); auto. }
 
-      pose proof (IHHT1 c H env0 env0' V).
-      unfold LR in H0. destruct H0 as [_ [_ [v1 [v1' [Hsnf [Hsnf' Hdv1]]]]]].
+      pose proof (IHHT1 c H0 env0 env0' V).
+      unfold LR in H1. destruct H1 as [_ [_ [v1 [v1' [Hsnf [Hsnf' Hdv1]]]]]].
       inversion Hty; inversion Hty'; subst.
-      pose proof (wt_nf_is_value _ _ _ H7 Hsnf); clear H8 H9.
-      pose proof (wt_nf_is_value' _ _ _ H17 Hsnf'); clear H18 H19.
+      pose proof (wt_nf_is_value _ _ _ H8 Hsnf); clear H9 H10.
+      pose proof (wt_nf_is_value' _ _ _ H18 Hsnf'); clear H19 H20.
       destruct Hsnf as [Hms _]. destruct Hsnf' as [Hms' _].
       eapply mstep_mstep'__preserves_LR'.
       exact Hty. exact Hty'.
       eapply multistep_case1; eassumption.
       eapply multistep'_case1'; eassumption.
-      pose proof (preservation_multi _ _ _ H7 Hms).
-      pose proof (preservation'_multi _ _ _ H17 Hms').
-      clear H7 H17.
+      pose proof (preservation_multi _ _ _ H8 Hms).
+      pose proof (preservation'_multi _ _ _ H18 Hms').
+      clear H8 H18.
 
-      pose proof (related_canonical_forms_list v1 v1' H2 H3 H0 H1).
-      destruct H4. exists cfg; auto. clear H2 H3.
+      pose proof (related_canonical_forms_list v1 v1' H3 H4 H1 H2).
+      destruct H5. exists cfg; auto. clear H3 H4.
       (* Case Nil *)
-      { destruct H4; subst. clear H0 H1 Hdv1 Hms Hms'.
+      { destruct H5; subst. clear H1 H2 Hdv1 Hms Hms'.
         eapply mstep_mstep'__preserves_LR'.
         inversion Hty; subst.
         constructor; eauto.
@@ -825,7 +824,7 @@ Proof.
         apply multi_refl.
         eapply IHHT2; auto. }
       (* Case Cons *)
-      { destruct H4 as [v2 [v3 [v2' [v3' [Hv2' [Hv3' [Hv2 [Hv3 [Heq Heq']]]]]]]]].
+      { destruct H5 as [v2 [v3 [v2' [v3' [Hv2' [Hv3' [Hv2 [Hv3 [Heq Heq']]]]]]]]].
         subst. eapply mstep_mstep'__preserves_LR'.
         inversion Hty; subst.
         constructor; eauto.
@@ -848,35 +847,35 @@ Proof.
           destruct (String.eqb x s); auto;
           destruct (String.eqb y s); auto.
         - repeat constructor; auto.
-          inversion H2; subst; auto.
           inversion H3; subst; auto.
+          inversion H4; subst; auto.
           apply simpl_derive'_list in Hdv1 as [Hdv2 Hdv3].
           exists v3, v3'. repeat split; auto.
           apply value_is_nf; auto.
           apply value'_is_nf; auto.
-          inversion H2; subst; auto.
           inversion H3; subst; auto.
+          inversion H4; subst; auto.
           apply simpl_derive'_list in Hdv1 as [Hdv2 Hdv3].
           exists v2, v2'. repeat split; auto.
           apply value_is_nf; auto.
           apply value'_is_nf; auto.
         - eapply typable_empty__closed'.
-          inversion H3; subst; eauto.
+          inversion H4; subst; eauto.
         - eapply instantiation_env_closed. eassumption.
         - eapply typable_empty__closed'.
-          inversion H3; subst; eauto.
+          inversion H4; subst; eauto.
         - eapply instantiation_env_closed.
           eapply instantiation_drop. eassumption.
         - eapply typable_empty__closed.
-          inversion H2; subst; eauto.
+          inversion H3; subst; eauto.
         - eapply instantiation_env_closed. eassumption.
         - eapply typable_empty__closed.
-          inversion H2; subst; eauto.
+          inversion H3; subst; eauto.
         - eapply instantiation_env_closed.
           eapply instantiation_drop. eassumption. }
 Qed.
 
-Theorem commutativity: forall T cfg analysis,
+Theorem commutativity `{NatOp}: forall T cfg analysis,
   base_ty T ->
   has_type empty analysis (Arrow T T) ->
   commutes T cfg analysis.
