STLC_SuccNat/Derivation.v
@@ -134,11 +134,11 @@ Fixpoint term_derivation (cfg : feat_config) (t' : tm') : option tm :=
                 | None => None
                 | Some t => Some (succ t)
                 end
-  | add' t1' t2' => match term_derivation cfg t1' with
+  | op' t1' t2' => match term_derivation cfg t1' with
                     | None => None
                     | Some t1 => match term_derivation cfg t2' with
                                  | None => None
-                                 | Some t2 => Some (add t1 t2)
+                                 | Some t2 => Some (op t1 t2)
                                  end
                     end
   | nil' => Some nil
